

## Lecture 4

CDF of  $X, Y$  (RVs)

$$F_{XY}(x, y) = P(X \leq x \cap Y \leq y) = P(X \leq x, Y \leq y)$$

$$\{\omega \in \Omega : X(\omega) \leq x\} \cap \{\omega \in \Omega : Y(\omega) \leq y\}$$

### Properties

1. Limits:

$$\lim_{x, y \rightarrow \infty} F_{XY}(x, y) = 1$$

$$\lim_{x \rightarrow -\infty} F_{XY}(x, y) = 0, \quad \forall y \in \mathbb{R}$$

vice versa

$$\begin{aligned} \lim_{x \rightarrow \infty} F_{XY}(x, y) &= \lim_{x \rightarrow \infty} P(X \leq x \cap Y \leq y) = P(\Omega \cap Y \leq y) = P(Y \leq y) \\ &= F_Y(y) \quad (\text{marginal cdf}) \end{aligned}$$

2.  $F_{XY}$  is non-decreasing in  $x, y$

3.  $F_{XY}$  is right-continuous in  $x, y$

## Bivariate PMF

Recall  $f_X(x) = P(X=x)$

$$f_{XY}(x,y) = P(X=x, Y=y)$$

$$F_{XY}(x,y) = \sum_{x' \leq x} \sum_{y' \leq y} f_{XY}(x',y')$$

X		Y			
		1	2	3	$f_X(x)$
	0	0.2	0.1	0.2	0.5
	1	0.3	0.1	0.1	0.5
	$f_Y(y)$	0.5	0.2	0.3	

$f_X(x) = \sum_y f_{XY}(x,y)$   
 $\sum_x \sum_y f_{XY}(x,y) = 1$

## Bivariate PDF

$X, Y$  are jointly continuous, the PDF is an integrable function

$$F_{XY}(x,y) = \int_{-\infty}^x \int_{-\infty}^y f_{XY}(x,y) dx dy$$

1.  $f_{XY}(x,y) \geq 0 \quad \forall x,y \in \mathbb{R}$

2.  $\int_{-\infty}^{\infty} \int_{-\infty}^{\infty} f_{XY}(x,y) dx dy = 1$

3.  $P((X,Y) \in B) = \iint_B f_{XY}(x,y) dx dy$

$$f_{XY}(x,y) = \frac{\partial^2}{\partial x \partial y} F_{XY}(x,y)$$

$$f_X(x) = \int_{-\infty}^{\infty} f_{XY}(x,y) dy, \text{ viceversa}$$


---

### Joint Moments

$X, Y$  are RVs

$g(X,Y)$  is also a RV if  $g$  is "nice"

$$\mathbb{E}[g(X,Y)] = \begin{cases} \sum_x \sum_y g(x,y) f_{XY}(x,y) & \text{discrete} \\ \int_{-\infty}^{\infty} \int_{-\infty}^{\infty} g(x,y) f_{XY}(x,y) dx dy & \text{continuous} \end{cases}$$

Suppose  $X$  is discrete

$$\mathbb{E}[g(X,Y)] = \sum_x \int_{-\infty}^{\infty} g(x,y) f_{XY}(x,y) dy$$

## Covariance

$$\text{Cov}(X, Y) = \mathbb{E}[(X - \mathbb{E}[X])(Y - \mathbb{E}[Y])] = \mathbb{E}[XY] - \mathbb{E}[X]\mathbb{E}[Y]$$

$$\text{Cov}(X, Y) = \text{Cov}(Y, X)$$

$$\text{Cov}(aX, Y) = a \text{Cov}(X, Y)$$

$$\text{Cov}(X+Z, Y) = \text{Cov}(X, Y) + \text{Cov}(Z, Y)$$

$$\text{Cov}(X, X) = \text{Var}(X)$$

$$\begin{aligned}\text{Var}(X+Y) &= \mathbb{E}[(X+Y)^2] - \mathbb{E}[X+Y]^2 \\ &= \text{Var}(X) + \text{Var}(Y) + 2\mathbb{E}[XY] - 2\mathbb{E}[X]\mathbb{E}[Y] \\ &\quad + 2\text{Cov}(X, Y)\end{aligned}$$

$$\text{Corr}(X, Y) = \frac{\text{Cov}(X, Y)}{\sqrt{\text{Var}(X) \text{Var}(Y)}}$$

$$|\text{Corr}(X, Y)| \leq 1$$

$$|\text{Corr}(X, Y)| = 1 \quad \text{if and only if} \quad Y = a + bX, \quad a, b \in \mathbb{R}$$

## Independence

$$X \perp Y \iff \{X \leq x\} \overset{\text{mutually}}{\perp} \{Y \leq y\} \quad \forall x, y \in \mathbb{R}$$

$$P(A \cap B) = P(A)P(B), \quad A \perp B$$

$$F_{XY}(x, y) = F_X(x) F_Y(y)$$

Equivalently:  $f_{XY}(x, y) = f_X(x) f_Y(y)$

Example:  $X \perp Y$  and cts

$$E[XY] = \int_{-\infty}^{\infty} \int_{-\infty}^{\infty} xy f_{XY}(x, y) dx dy$$

$$= \int_{-\infty}^{\infty} \int_{-\infty}^{\infty} xy f_X(x) f_Y(y) dx dy$$

$$= \int_{-\infty}^{\infty} y f_Y(y) \left( \int_{-\infty}^{\infty} x f_X(x) dx \right) dy$$

$$= E[X] \int_{-\infty}^{\infty} y f_Y(y) dy = E[X] E[Y]$$

$$\Rightarrow \text{if } X \perp Y \quad \text{Cov}(X, Y) = 0$$

Suppose  $g(X, Y) = h(X)k(Y)$

$$X \perp Y: \mathbb{E}[g(X, Y)] = \mathbb{E}[h(X)] \mathbb{E}[k(Y)]$$

$$\mathbb{E}[e^{tx+uy}] = \mathbb{E}[e^{tx}] \mathbb{E}[e^{uy}] = M_X(t) M_Y(u)$$

---

Sums of RVs

$$Z = X + Y$$

$$f_Z(z) = \begin{cases} \sum_u f_{XY}(u, z-u) & \text{discrete} \\ \int_{-\infty}^{\infty} f_{XY}(u, z-u) du & \text{cts} \end{cases}$$

Proof (Discrete)

$$\{Z=z\} \quad Z = X + Y$$

$$\{Z=z\} = \bigcup_u \{X=u, Y=z-u\}$$

$$P(Z=z) = \sum_u P(X=u, Y=z-u) = \sum_u f_{XY}(u, z-u)$$

$$g \perp Y, Z = X + Y$$

$$f_Z(z) = \begin{cases} \sum_u f_X(u) f_Y(z-u) \\ \int_{-\infty}^{\infty} f_X(u) f_Y(z-u) du \end{cases}$$

"Convolution of  $X$  and  $Y$ "

$$f_Z = f_X * f_Y$$

$$\underset{n \times 1}{X} : \Omega \rightarrow \mathbb{R}^n$$

$$\text{Var}(\underset{n \times 1}{X}) = \mathbb{E} \left[ \left( \underset{n \times 1}{X} - \underset{n \times 1}{\mathbb{E}[X]} \right) \left( \underset{n \times 1}{X} - \underset{n \times 1}{\mathbb{E}[X]} \right)^T \right] = \text{cylinder}$$

$$= \begin{pmatrix} \text{Var}(X_1) & \text{Cov}(X_1, X_2) & \dots & \text{Cov}(X_1, X_n) \\ \text{Cov}(X_2, X_1) & \ddots & & \vdots \\ \vdots & & \ddots & \vdots \\ \text{Cov}(X_n, X_1) & \dots & \dots & \text{Var}(X_n) \end{pmatrix}$$

If  $X_i$ 's are independent then  $\text{Var}(X)$  is diagonal

identically distributed with  $\text{Var}(X_i) = \sigma^2$ ,  $\text{Var}(X) = \sigma^2 I_{n \times n}$

$\text{Var}(X)$  is PSD  $\Leftrightarrow \forall a \in \mathbb{R}^m \quad a^T \text{Var}(X) a \geq 0$ ,

Proof:  $0 \leq \text{Var}(a^T X) = \mathbb{E} \left[ (a^T X - \mathbb{E}[a^T X]) (a^T X - \mathbb{E}[a^T X])^T \right] / (a^T X - \mathbb{E}[a^T X])^T$

$$= \mathbb{E} \left[ a^T (X - \mathbb{E}[X]) (X - \mathbb{E}[X])^T a \right]$$

$$= a^T \text{Var}(X) a$$


---

### Conditional Distribution

$$P(B) > 0, \quad P(A|B) = \frac{P(A \cap B)}{P(B)}$$

The PDF/PMF of  $Y$  given  $X=x$  is given

$$f_{Y|X}(y|x) = \frac{f_{XY}(x,y)}{f_X(x)}$$

Is this valid?

$$\sum_y f_{Y|X}(y|x) = \sum_y \frac{f_{XY}(x,y)}{f_X(x)} = \frac{1}{f_X(x)} \sum_y f_{XY}(x,y)$$

$$= 1$$

$$F_{Y|X}(y|x) = \begin{cases} \sum_{y' \leq y} f_{Y|X}(y'|x) \\ \int_{-\infty}^y f_{Y|X}(y'|x) dy' \end{cases}$$

## Hurricanes

$Y$  # hurricanes reaching land

$N$  # hurricanes formed in ocean

$$Y|N=n \sim \text{Bin}(n, p) \quad \mathbb{E}[Y|N=n] = np$$

$$N \sim \text{Poisson}(\lambda) \quad \mathbb{E}[N] = \lambda$$

One can show  $Y \sim \text{Poisson}(\lambda p)$

---

## Conditional Expectation

The conditional expectation of  $Y$  given  $X=x$

$$\mathbb{E}[Y|X=x] = \begin{cases} \sum_y y f_{Y|X}(y|x) & \text{discrete} \\ \int_{-\infty}^{\infty} y f_{Y|X}(y|x) & \text{cts} \end{cases}$$

$$\psi(x) = \mathbb{E}[Y|X=x]$$

The conditional expectation of  $Y$  given  $X$  is  $\psi(X)$  and we write

$$\mathbb{E}[Y|X]$$

Law of Total Expectations:

$$E[E[Y|X]] = E[Y]$$

Proof:

$$\begin{aligned} & \int_{-\infty}^{\infty} E[Y|X=x] f_X(x) dx \\ &= \int_{-\infty}^{\infty} \int_{-\infty}^{\infty} y f_{Y|X}(y|x) dy f_X(x) dx \quad \left| \quad f_{Y|X}(y|x) = \frac{f_{XY}(x,y)}{f_X(x)} \right. \\ &= \int_{-\infty}^{\infty} y \int_{-\infty}^{\infty} f_{XY}(x,y) dx dy \\ &= \int_{-\infty}^{\infty} y f_Y(y) dy = E[Y] \end{aligned}$$

---

$$g(X,Y) = h(X)k(Y)$$

$$\# \quad E[g(X,Y) | X=x] = h(x) E[k(Y) | X=x]$$

$$E[g(X,Y) | X] = h(X) E[k(Y) | X]$$